examples/map/MapI0Mproof.v
@@ -17,7 +17,7 @@ From ExtLib Require Import
      Data.Map.FMapAList.
 Require Import HTactics ProofMode IPM.
 Require Import OpenDef.
-Require Import Mem1 MemOpen STB.
+Require Import Mem1 MemOpen STB Invariant.
 
 Set Implicit Arguments.
 
@@ -33,21 +33,13 @@ Section SIMMODSEM.
 
   Let W: Type := Any.t * Any.t.
 
-  From iris.algebra Require Import big_op.
-  From iris.bi Require Import big_op.
-
   Let wf: _ -> W -> Prop :=
-    @mk_wf _ unit
-           (fun _ _stk_mgr0 _ =>
-              ⌜True⌝ ** (∃ (stk_mgr0: gmap mblock (list val)),
-                         (⌜_stk_mgr0 = stk_mgr0↑⌝) ∧
-                         ({{"SIM": ([∗ map] handle ↦ stk ∈ stk_mgr0,
-                                    (∃ hd, OwnM ((handle, 0%Z) |-> [hd]) ** is_list hd stk))}})
-           ))
-  .
+        @mk_wf _ unit
+               (fun _ st_src st_tgt =>
+                  ((∃ blk ofs l, ⌜st_src = l↑ /\ st_tgt = (Vptr blk ofs)↑⌝ ** OwnM ((blk, ofs) |-> (List.map Vint l)) ** pending0) ∨ (⌜st_src = ([]: list Z)↑⌝))%I).
 
-  Variable global_stb: gname -> option fspec.
-  Hypothesis STBINCL: stb_incl (to_stb (StackStb ++ MemStb)) global_stb.
+  Variable GlobalStb: Sk.t -> gname -> option fspec.
+  Hypothesis STBINCL: forall sk, stb_incl (to_stb MemStb) (GlobalStb sk).
 
   Ltac renamer :=
     match goal with
@@ -71,7 +63,190 @@ Section SIMMODSEM.
       astep fn (tt↑)
     end.
 
-  Theorem sim_modsem: ModSemPair.sim (Stack1.StackSem global_stb) Stack0.StackSem.
+  Lemma pending0_unique:
+    pending0 -∗ pending0 -∗ False%I.
+  Proof.
+    iIntros "H0 H1". iCombine "H0 H1" as "H".
+    iOwnWf "H". exfalso. rr in H1. clear - H1. admit "ez".
+  Qed.
+
+  Lemma points_to_get_split blk ofs l k v
+        (GET: nth_error l k = Some v)
+    :
+    OwnM((blk, ofs) |-> l) -∗ (OwnM((blk, (ofs + k)%Z) |-> [v])) ** ((OwnM((blk, (ofs + k)%Z) |-> [v]) -* OwnM((blk, ofs) |-> l))).
+  Proof.
+    revert blk ofs k v GET. induction l; ss; i.
+    { destruct k; ss. }
+    destruct k; ss.
+    { clarify. iIntros "H". rewrite points_to_split.
+      iDestruct "H" as "[H0 H1]". iSplitL "H0".
+      { rewrite Z.add_0_r. ss. }
+      iIntros "H". iSplitL "H".
+      { rewrite Z.add_0_r. ss. }
+      { ss. }
+    }
+    { iIntros "H". rewrite points_to_split.
+      iDestruct "H" as "[H0 H1]".
+      iPoseProof (IHl with "H1") as "H1"; eauto.
+      iDestruct "H1" as "[H1 H2]".
+      replace (ofs + Z.pos (Pos.of_succ_nat k))%Z with (ofs + 1 + k)%Z by lia.
+      iSplitL "H1"; auto. iIntros "H1". iSplitL "H0"; auto.
+      iApply "H2". auto.
+    }
+  Qed.
+
+  Lemma points_to_set_split blk ofs l k v l'
+        (GET: set_nth k l v = Some l')
+    :
+    OwnM((blk, ofs) |-> l) -∗ (∃ v', OwnM((blk, (ofs + k)%Z) |-> [v'])) ** ((OwnM((blk, (ofs + k)%Z) |-> [v]) -* OwnM((blk, ofs) |-> l'))).
+  Proof.
+    revert blk ofs k v l' GET. induction l; ss; i.
+    { destruct k; ss. }
+    destruct k; ss.
+    { clarify. iIntros "H". rewrite points_to_split.
+      iDestruct "H" as "[H0 H1]". iSplitL "H0".
+      { rewrite Z.add_0_r. iExists _. ss. }
+      iIntros "H". iEval (rewrite points_to_split). iSplitL "H".
+      { rewrite Z.add_0_r. ss. }
+      { ss. }
+    }
+    { iIntros "H". rewrite points_to_split.
+      iDestruct "H" as "[H0 H1]".
+      unfold option_map in GET. des_ifs.
+      iPoseProof (IHl with "H1") as "H1"; eauto.
+      iDestruct "H1" as "[H1 H2]". iDestruct "H1" as (v') "H1".
+      replace (ofs + Z.pos (Pos.of_succ_nat k))%Z with (ofs + 1 + k)%Z by lia.
+      iSplitL "H1"; auto. iIntros "H1".
+      iEval (rewrite points_to_split). iSplitL "H0"; auto.
+      iApply "H2". auto.
+    }
+  Qed.
+
+  Theorem correct: refines2 [MapI0.Map] [MapM.Map GlobalStb].
+  Proof.
+    eapply adequacy_local2. econs; ss. i. rr.
+    econstructor 1 with (wf:=wf) (le:=top2); ss; et; swap 2 3.
+    { esplits. rr. econs; ss. eapply to_semantic. iIntros "_". iRight. auto. }
+    econs; ss.
+    { unfold MapI0.initF, MapM.initF, ccallU. init. harg. mDesAll. subst.
+      mDesOr "INV".
+      { mDesAll. subst. mAssertPure False; ss. iApply (pending0_unique with "A1 A"). }
+      mDesAll. subst. steps. astart 100. acatch.
+      { eapply STBINCL. stb_tac. ss. }
+      hcall _ _ with "".
+      { iModIntro. iSplitL.
+        { iRight. ss. }
+        instantiate (1:=Some _). ss. iPureIntro.
+        splits; ss. admit "add range condition".
+      }
+      { ss. }
+      ss. mDesAll. subst.
+      { mDesOr "INV".
+        { mDesAll. subst. mAssertPure False; ss. iApply (pending0_unique with "A2 A"). }
+        mDesAll. subst. steps. astop. steps.
+        hret _; ss.
+        iModIntro. iSplit.
+        { iLeft. iSplits. iSplitR "A"; eauto. iSplit; eauto.
+          admit "malloc -> calloc".
+        }
+        { iSplits; eauto. }
+      }
+    }
+    econs; ss.
+    { unfold MapI0.setF, MapM.setF, ccallU. init. harg. mDesAll. subst.
+      mDesOr "INV".
+      2:{ mDesAll. subst. steps. astop. steps. des_ifs. }
+      mDesAll. des. steps. unfold scale_int. des_ifs.
+      2:{ admit "add int allignment condition". }
+      steps. astart 1. acatch.
+      { eapply STBINCL. stb_tac. ss. }
+      hcall _ _ with "".
+      { iModIntro. iSplitR.
+        { iLeft. ss. }
+        instantiate (1:=Some _). ss. iPureIntro.
+        splits; ss. admit "add range condition".
+      }
+      { ss. }
+      ss. mDesAll. subst.
+      { mDesOr "INV".
+        { mDesAll. subst. mAssertPure False; ss. iApply (pending0_unique with "A2 A"). }
+        mDesAll. subst. steps. astop. steps.
+        hret _; ss.
+        iModIntro. iSplit.
+        { iLeft. iSplits. iSplitR "A"; eauto. iSplit; eauto.
+          admit "malloc -> calloc".
+        }
+        { iSplits; eauto. }
+      }
+
+steps. .ired_l. _step.
+      { ired_both. _step. des_ifs_safe. steps. force_l. steps.
+
+ force_l. force_r.
+      {
+
+subst. steps. astop. steps. ired_l. steps. force_l. force_r.
+      {
+
+      subst. force_r. _step. steps. astart 10. steps.
+
+red in WF. inv WF.
+
+astop. steps. des_ifs. }
+
+
+    }
+
+mDesAll. subst. mAssertPure False; ss. iApply (pending0_unique with "A1 A"). }
+      mDesAll. subst. steps. astart 100. acatch.
+      { eapply STBINCL. stb_tac. ss. }
+      hcall _ _ with "".
+      { iModIntro. iSplitL.
+        { iRight. ss. }
+        instantiate (1:=Some _). ss. iPureIntro.
+        splits; ss. admit "add range condition".
+      }
+      { ss. }
+      ss. mDesAll. subst.
+      { mDesOr "INV".
+        { mDesAll. subst. mAssertPure False; ss. iApply (pending0_unique with "A2 A"). }
+        mDesAll. subst. steps. astop. steps.
+        hret _; ss.
+        iModIntro. iSplit.
+        { iLeft. iSplits. iSplitR "A"; eauto. iSplit; eauto.
+          admit "malloc -> calloc".
+        }
+        { iSplits; eauto. }
+      }
+    }
+    {
+
+
+iSplits; eauto.
+iLeft.
+
+        { mDe
+
+
+eauto. eauto.
+
+        {
+
+
+      }
+
+
+stbtac.
+
+steps.
+      hcall _ _ with "".
+
+      unfold
+ss.
+
+
+
+ sim_modsem: ModSemPair.sim MapM.MapSem (Stack1.StackSem global_stb) Stack0.StackSem.
   Proof.
     econstructor 1 with (wf:=wf) (le:=top2); ss; et; swap 2 3.
     { esplits. econs; ss. eapply to_semantic. iIntros "H". iClear "H". iSplits; ss. }
